The Great Refactor, part two

Hashmap/DHashMap/AdditionalOperations.lean
@@ -18,10 +18,10 @@ variable {α : Type u} {β : α → Type v} {γ : Type w} {δ : α → Type w}
 
 namespace MyLean.DHashMap
 
-def filterMap [BEq α] [Hashable α] (f : (a : α) → β a → Option (δ a)) (m : DHashMap α β) : DHashMap α δ :=
+@[specialize, inline] def filterMap [BEq α] [Hashable α] (f : (a : α) → β a → Option (δ a)) (m : DHashMap α β) : DHashMap α δ :=
   ⟨Raw₀.filterMap f ⟨m.1, m.2.size_buckets_pos⟩, .wf (Raw₀.filterMap f ⟨m.1, m.2.size_buckets_pos⟩).2 m.2.out.filterMap⟩
 
-def map [BEq α] [Hashable α] (f : (a : α) → β a → δ a) (m : DHashMap α β) : DHashMap α δ :=
+@[specialize, inline] def map [BEq α] [Hashable α] (f : (a : α) → β a → δ a) (m : DHashMap α β) : DHashMap α δ :=
   ⟨Raw₀.map f ⟨m.1, m.2.size_buckets_pos⟩, .wf (Raw₀.map f ⟨m.1, m.2.size_buckets_pos⟩).2 m.2.out.map⟩
 
 end MyLean.DHashMap
