Hashmap/HashSet/Basic.lean
@@ -26,15 +26,30 @@ namespace Raw
 instance : EmptyCollection (Raw α) where
   emptyCollection := empty
 
+@[inline] def insert [BEq α] [Hashable α] (m : Raw α) (a : α) : Raw α :=
+  ⟨m.inner.insert a ()⟩
+
 @[inline] def containsThenInsert [BEq α] [Hashable α] (m : Raw α) (a : α) : Raw α × Bool :=
   let ⟨r, replaced⟩ := m.inner.containsThenInsert a ()
   ⟨⟨r⟩, replaced⟩
 
-@[inline] def insert [BEq α] [Hashable α] (m : Raw α) (a : α) : Raw α :=
-  ⟨m.inner.insert a ()⟩
-
 @[inline] def contains [BEq α] [Hashable α] (m : Raw α) (a : α) : Bool :=
   m.inner.contains a
+
+instance [BEq α] [Hashable α] : Membership α (Raw α) where
+  mem a m := m.contains a
+
+@[inline] def remove [BEq α] [Hashable α] (m : Raw α) (a : α) : Raw α :=
+  ⟨m.inner.remove a⟩
+
+@[inline] def filter [BEq α] [Hashable α] (f : α → Bool) (m : Raw α) : Raw α :=
+  ⟨m.inner.filter fun a _ => f a⟩
+
+@[inline] def foldlM {m : Type v → Type v} [Monad m] {β : Type v} (f : β → α → m β) (init : β) (b : Raw α) : m β :=
+  b.inner.foldlM (fun b a _ => f b a) init
+
+@[inline] def foldl {β : Type v} (f : β → α → β) (init : β) (m : Raw α) : β :=
+  m.inner.foldl (fun b a _ => f b a) init
 
 @[inline] def size (m : Raw α) : Nat :=
   m.inner.size
@@ -51,11 +66,17 @@ theorem WF.empty [BEq α] [Hashable α] {c} : (empty c : Raw α).WF :=
 theorem WF.emptyc [BEq α] [Hashable α] : (∅ : Raw α).WF :=
   HashMap.Raw.WF.empty
 
+theorem WF.insert [BEq α] [Hashable α] {m : Raw α} {a : α} (h : m.WF) : (m.insert a).WF :=
+  HashMap.Raw.WF.insert h
+
 theorem WF.containsThenInsert [BEq α] [Hashable α] {m : Raw α} {a : α} (h : m.WF) : (m.containsThenInsert a).1.WF :=
   HashMap.Raw.WF.containsThenInsert h
 
-theorem WF.insert [BEq α] [Hashable α] {m : Raw α} {a : α} (h : m.WF) : (m.insert a).WF :=
-  HashMap.Raw.WF.insert h
+theorem WF.remove [BEq α] [Hashable α] {m : Raw α} {a : α} (h : m.WF) : (m.remove a).WF :=
+  HashMap.Raw.WF.remove h
+
+theorem WF.filter [BEq α] [Hashable α] {m : Raw α} {f : α → Bool} (h : m.WF) : (m.filter f).WF :=
+  HashMap.Raw.WF.filter h
 
 end Raw
 
@@ -72,15 +93,30 @@ namespace HashSet
 instance [BEq α] [Hashable α] : EmptyCollection (HashSet α) where
   emptyCollection := empty
 
+@[inline] def insert [BEq α] [Hashable α] (m : HashSet α) (a : α) : HashSet α :=
+  ⟨m.inner.insert a ()⟩
+
 @[inline] def containsThenInsert [BEq α] [Hashable α] (m : HashSet α) (a : α) : HashSet α × Bool :=
   let ⟨r, replaced⟩ := m.inner.containsThenInsert a ()
   ⟨⟨r⟩, replaced⟩
 
-@[inline] def insert [BEq α] [Hashable α] (m : HashSet α) (a : α) : HashSet α :=
-  ⟨m.inner.insert a ()⟩
-
 @[inline] def contains [BEq α] [Hashable α] (m : HashSet α) (a : α) : Bool :=
   m.inner.contains a
+
+instance [BEq α] [Hashable α] : Membership α (HashSet α) where
+  mem a m := m.contains a
+
+@[inline] def remove [BEq α] [Hashable α] (m : HashSet α) (a : α) : HashSet α :=
+  ⟨m.inner.remove a⟩
+
+@[inline] def filter [BEq α] [Hashable α] (f : α → Bool) (m : HashSet α) : HashSet α :=
+  ⟨m.inner.filter fun a _ => f a⟩
+
+@[inline] def foldlM [BEq α] [Hashable α] {m : Type v → Type v} [Monad m] {β : Type v} (f : β → α → m β) (init : β) (b : HashSet α) : m β :=
+  b.inner.foldlM (fun b a _ => f b a) init
+
+@[inline] def foldl [BEq α] [Hashable α] {β : Type v} (f : β → α → β) (init : β) (m : HashSet α) : β :=
+  m.inner.foldl (fun b a _ => f b a) init
 
 @[inline] def size [BEq α] [Hashable α] (m : HashSet α) : Nat :=
   m.inner.size
