Hashmap/HashMap/AdditionalOperations.lean
@@ -1,0 +1,37 @@
+/-
+Copyright (c) 2024 Lean FRO, LLC. All rights reserved.
+Released under Apache 2.0 license as described in the file LICENSE.
+Authors: Markus Himmel
+-/
+import Hashmap.DHashMap.AdditionalOperations
+import Hashmap.HashMap.Basic
+
+set_option autoImplicit false
+
+universe u v w
+
+variable {α : Type u} {β : Type v} {γ : Type w}
+
+namespace MyLean
+
+namespace HashMap
+
+namespace Raw
+
+theorem WF.filterMap [BEq α] [Hashable α] {m : Raw α β} {f : α → β → Option γ} (h : m.WF) : (m.filterMap f).WF :=
+  DHashMap.Raw.WF.filterMap h
+
+theorem WF.map [BEq α] [Hashable α] {m : Raw α β} {f : α → β → γ} (h : m.WF) : (m.map f).WF :=
+  DHashMap.Raw.WF.map h
+
+end Raw
+
+@[specialize, inline] def filterMap [BEq α] [Hashable α] (f : α → β → Option γ) (m : HashMap α β) : HashMap α γ :=
+  ⟨m.inner.filterMap f⟩
+
+@[specialize, inline] def map [BEq α] [Hashable α] (f : α → β → γ) (m : HashMap α β) : HashMap α γ :=
+  ⟨m.inner.map f⟩
+
+end HashMap
+
+end MyLean
